lawyer/nonblocking/wptp_gen.v
@@ -1,0 +1,302 @@
+From iris.proofmode Require Import tactics.
+From iris.base_logic Require Import iprop. 
+From trillium.program_logic Require Import adequacy_utils. 
+From heap_lang Require Import lang locales_helpers_hl.
+From fairness Require Import locales_helpers.
+
+Close Scope Z.
+
+
+Section WptpGen.
+  Context {Σ: gFunctors}.
+  Context (W: expr -> locale heap_lang -> (val → iPropI Σ) -> iProp Σ).
+  
+  Definition wptp_from_gen 
+    (t0 t: list expr) (Φs : list (val → iPropI Σ)) :=
+    ([∗ list] tp1_e;Φ ∈ (prefixes_from t0 t);Φs,
+       W tp1_e.2 (locale_of tp1_e.1 tp1_e.2) Φ)%I.
+
+  Lemma wptp_from_gen_app' t0 t1 Φs1 t2 Φs2
+    (MATCH1: length t1 = length Φs1):
+    wptp_from_gen t0 (t1 ++ t2) (Φs1 ++ Φs2) ⊢ wptp_from_gen t0 t1 Φs1 ∗ wptp_from_gen (t0 ++ t1) t2 Φs2. 
+  Proof using.
+    iIntros.
+    rewrite {1}/wptp_from_gen. rewrite prefixes_from_app. 
+    iDestruct (big_sepL2_app_inv with "[$]") as "(?&?)".
+    2: { iFrame. }
+    rewrite prefixes_from_length. tauto.  
+  Qed.
+
+  Lemma wptp_from_gen_app t0 t1 Φs1 t2 Φs2:
+    wptp_from_gen t0 t1 Φs1 ∗ wptp_from_gen (t0 ++ t1) t2 Φs2 ⊢
+      wptp_from_gen t0 (t1 ++ t2) (Φs1 ++ Φs2). 
+  Proof using.
+    iIntros "[WPS1 WPS2]".
+    rewrite {3}/wptp_from_gen. rewrite prefixes_from_app.
+    iDestruct (big_sepL2_length with "WPS1") as "%".
+    iApply big_sepL2_app_same_length; [tauto| ].
+    iFrame. 
+  Qed.
+
+  Lemma wptp_gen_split_1 t0 t1 t2 Φs:
+    wptp_from_gen t0 (t1 ++ t2) Φs ⊢
+      ⌜ exists Φs1 Φs2, Φs1 ++ Φs2 = Φs /\ length Φs1 = length t1 /\ length Φs2 = length t2 ⌝.
+  Proof using.
+    clear. 
+    iIntros "WPS".
+    iDestruct (big_sepL2_length with "[$]") as "%LENS".
+    rewrite adequacy_utils.prefixes_from_length in LENS.
+    iPureIntro.
+    do 2 eexists. split.
+    { apply (take_drop (length t1)). }
+    rewrite length_take. rewrite length_skipn.
+    rewrite length_app in LENS. lia.
+  Qed.
+
+  Lemma wptp_gen_singleton t0 e Φ:
+    wptp_from_gen t0 [e] [Φ] ⊣⊢ W e (locale_of t0 e) Φ. 
+  Proof using.
+    rewrite /wptp_from_gen. simpl.
+    by rewrite bi.sep_emp.
+  Qed.
+
+  Lemma new_threads_wptp_from_gen `{!irisG heap_lang M Σ} t efs:
+    ([∗ list] i ↦ ef ∈ efs, 
+      W ef (locale_of (t ++ take i efs) ef) (fork_post (locale_of (t ++ take i efs) ef))
+    )
+      ⊣⊢ wptp_from_gen t efs (newposts t (t ++ efs)).
+  Proof.
+    rewrite  /wptp_from_gen. 
+    rewrite big_sepL2_alt; iSplit.
+    - iIntros "H". iSplit.
+      { rewrite /newposts. rewrite map_length.
+        rewrite /newelems. rewrite drop_app_length // map_length !prefixes_from_length //. }
+      iInduction efs as [|ef efs] "IH" forall (t); first done.
+      rewrite /newposts /newelems.
+      rewrite /= !drop_app_length //=.
+      iDestruct "H" as "[H1 H]". rewrite (right_id [] (++)). iFrame.
+      replace (map (λ '(tnew, e), fork_post (locale_of tnew e))
+                 (prefixes_from (t ++ [ef]) efs))
+        with (newposts (t ++[ef]) ((t ++ [ef]) ++ efs)).
+      + iApply "IH". iApply (big_sepL_impl with "H").
+        iIntros "!>" (k e Hin) "H". by list_simplifier.
+      + list_simplifier.
+        replace (t ++ ef :: efs) with ((t ++ [ef]) ++ efs); last by list_simplifier.
+        rewrite /newposts /newelems.
+        rewrite drop_app_length //.
+    - iIntros "[_ H]".
+      iInduction efs as [|ef efs] "IH" forall (t); first done.
+      rewrite /newposts /newelems.
+      rewrite /= !drop_app_length //=.
+      iDestruct "H" as "[H1 H]". rewrite (right_id [] (++)). iFrame.
+      replace (map (λ '(tnew, e), fork_post (locale_of tnew e))
+                 (prefixes_from (t ++ [ef]) efs))
+          with (newposts (t ++[ef]) ((t ++ [ef]) ++ efs)).
+      + iSpecialize ("IH" with "H"). iApply (big_sepL_impl with "IH").
+        iIntros "!>" (k e Hin) "H". by list_simplifier.
+      + list_simplifier.
+        replace (t ++ ef :: efs) with ((t ++ [ef]) ++ efs); last by list_simplifier.
+        rewrite /newposts /newelems.
+        rewrite drop_app_length //.
+  Qed.
+
+  Lemma wptp_from_gen_cons t0 e efs Φ Φs:
+    wptp_from_gen t0 (e :: efs) (Φ :: Φs) ⊣⊢ W e (locale_of t0 e) Φ ∗ wptp_from_gen (t0 ++ [e]) efs Φs.
+  Proof using. done. Qed. 
+
+  (* TODO: do we need anything stronger (e.g. matching indices for e and Φ) ? *)
+  Lemma wptp_from_gen_take_2 t efs Φs τ
+    (IN: τ ∈ locales_of_list_from t efs):
+    let WPS := wptp_from_gen t efs Φs in
+    WPS ⊣⊢ ∃ Φ e, ⌜ Φ ∈ Φs ⌝ ∗ ⌜ from_locale_from t efs τ = Some e ⌝ ∗ W e τ Φ ∗ (W e τ Φ -∗ WPS).
+  Proof using.
+    simpl. iSplit. 
+    2: { iIntros "(%&%&?&?&?&CLOS)". by iApply "CLOS". }
+    iIntros "WPS".
+
+    pose proof IN as [e X]%locales_of_list_from_locale_from'.
+    apply from_locale_from_lookup in X. apply proj1 in X.
+    (* rewrite Nat.sub_0_r /= in X. *)
+    pose proof X as (t1 & t2 & -> & LEN)%elem_of_list_split_length. 
+
+    iDestruct (wptp_gen_split_1 with "[$]") as %(?&?&<-&?&?).
+    iDestruct (wptp_from_gen_app' with "[$]") as "[? WPS]"; eauto.
+    destruct x0; [done| ].
+    rewrite wptp_from_gen_cons. iDestruct "WPS" as "[WP ?]".
+
+    assert (length t ≤ τ).
+    { rewrite locales_of_list_from_indexes /= in IN.
+      apply elem_of_lookup_imap in IN as (?&?&?&?).
+      subst τ. clear.
+      simpl. lia. }
+
+    assert (from_locale_from t (t1 ++ e :: t2) τ = Some e) as E.
+    { eapply from_locale_from_lookup.
+      split; eauto. }
+    
+    do 2 iExists _. iSplit; [| iSplit].
+    2: done. 
+    { iPureIntro. Unshelve. 2: exact b. set_solver. }
+    assert (τ = locale_of (t ++ t1) e) as EQ.
+    2: { rewrite -EQ. iFrame.
+         iIntros. iApply wptp_from_gen_app. iFrame. simpl.
+         by rewrite -EQ. }
+    rewrite /locale_of. rewrite length_app.
+
+    (* lia.  *)
+    rewrite -LEN. by apply Nat.le_add_sub.     
+  Qed.
+
+  (* TODO: try to unify with wptp_from_gen_take_2 *)
+  (* TODO: do we need anything stronger (e.g. matching indices for e and Φ) ? *)
+  Lemma wptp_from_gen_take_1 t efs Φs e
+    (IN: e ∈ efs):
+    let WPS := wptp_from_gen t efs Φs in
+    WPS ⊣⊢ ∃ Φ t1 t2, let τ := locale_of (t ++ t1) e in
+       ⌜ Φ ∈ Φs ⌝ ∗ ⌜ efs = t1 ++ e :: t2 ⌝ ∗ W e τ Φ ∗ (W e τ Φ -∗ WPS).
+  Proof using.
+    simpl. iSplit.
+    2: { iIntros "(%&%&%&?&?&?&CLOS)". by iApply "CLOS". }
+    iIntros "WPS".    
+    apply elem_of_list_split in IN as (?&?&->).
+    iDestruct (wptp_gen_split_1 with "[$]") as %(?&?&<-&?&?).
+    iDestruct (wptp_from_gen_app' with "[$]") as "[? WPS]"; eauto.
+    destruct x2; [done| ].
+    rewrite wptp_from_gen_cons. iDestruct "WPS" as "[WP ?]".
+    do 3 iExists _. iSplit; [| iSplit].
+    2: { eauto. }
+    2: iFrame.
+    { iPureIntro. set_solver. }
+    iIntros "WP".
+    iApply wptp_from_gen_app. iFrame.
+  Qed.
+
+  (* EQUIV : locales_equiv t0 t0' *)
+
+  (* Lemma wptp_from_gen_locales_equiv_1_impl t0 t0' efs efs' Φs *)
+  (*   (EQUIV: locales_equiv_from t0 t0' efs efs'): *)
+  (*   wptp_from_gen t0 efs Φs -∗ wptp_from_gen t0' efs' Φs. *)
+  (* Proof using. *)
+  (*   iIntros "WPS".  *)
+  (*   (* rewrite /wptp_from_gen. *) *)
+  (*   (* iApply big_sepL2_proper_2. *) *)
+  (*   (* 4: by iFrame.  *) *)
+  (*   clear -EQUIV. *)
+  (*   Unset Printing Notations. *)
+    
+  (*   Disable Notation locales_equiv.  *)
+  (*   eapply EQUIV.  *)
+        
+  Lemma wptp_from_gen_locales_equiv_1 t0 t0' efs Φs
+    (EQUIV: locales_equiv t0 t0'):
+    wptp_from_gen t0 efs Φs ⊣⊢ wptp_from_gen t0' efs Φs.
+  Proof using.
+    generalize dependent Φs. generalize dependent t0. generalize dependent t0'.
+    induction efs.
+    { intros. simpl. set_solver. }
+    destruct Φs.
+    { set_solver. }
+    rewrite !wptp_from_gen_cons.
+    iApply bi.sep_proper.
+    2: { iApply IHefs.
+         clear -EQUIV.
+         rewrite !prefixes_from_app.
+         eapply Forall2_app; try done.
+         simpl. constructor; try done.
+         (* TODO: specific to heap_lang, can it be generalized? *)
+         rewrite /locale_of.
+         eapply adequacy_utils.locales_equiv_from_length; eauto. }
+    rewrite /locale_of.
+    eapply adequacy_utils.locales_equiv_from_length in EQUIV; eauto.
+    by rewrite EQUIV.
+  Qed.
+
+End WptpGen.
+
+
+  Lemma wptp_from_gen_upd_2 {Σ: gFunctors}
+    (W1 W2: expr -> locale heap_lang -> (val → iPropI Σ) -> iProp Σ) t efs Φs
+    (τs: gset (locale heap_lang))
+    (IN: τs ⊆ list_to_set $ locales_of_list_from t efs):
+    wptp_from_gen W1 t efs Φs -∗                  
+    (□ ∀ τ Φ e, ⌜ τ ∈ locales_of_list_from t efs /\ τ ∉ τs ⌝ -∗ W1 e τ Φ -∗ W2 e τ Φ) -∗
+    ∃ (M: gmap (locale heap_lang) (expr * (val → iPropI Σ))),
+    ⌜ dom M = τs ⌝ ∗
+    ([∗ map] τ ↦ '(e, Φ) ∈ M, (* ⌜ Φ ∈ Φs ⌝ ∗  *)⌜ from_locale_from t efs τ = Some e ⌝ ∗ W1 e τ Φ) ∗
+    (([∗ map] τ ↦ '(e, Φ) ∈ M, (* ⌜ Φ ∈ Φs ⌝ ∗  *)⌜ from_locale_from t efs τ = Some e ⌝ ∗ W2 e τ Φ) -∗ wptp_from_gen W2 t efs Φs).
+  Proof using.
+     iInduction efs as [|e efs] "IH" forall (Φs τs t IN). 
+     { simpl. iIntros "**".
+       apply equiv_empty_L in IN as ->.
+       iExists ∅. set_solver. }
+     iIntros "WPS #UPD".
+     assert (τs ∖ {[ locale_of t e ]} ⊆ list_to_set (locales_of_list_from (t ++ [e]) efs)).
+     { simpl in IN. set_solver. }
+
+     destruct Φs as [| Φ Φs]; [done| ].
+     rewrite wptp_from_gen_cons. iDestruct "WPS" as "[WP WPS]". 
+     
+     iSpecialize ("IH" with "[//] [$] []").
+     { iModIntro. iIntros "**". iApply ("UPD" with "[] [$]").
+       iPureIntro.
+       destruct H0.
+       rewrite locales_of_list_from_locales. simpl.
+       rewrite locales_of_list_from_locales in H0.
+       split; [set_solver| ].
+       apply not_elem_of_difference in H1 as [? | EQ]; [done| ].
+       apply elem_of_singleton in EQ.
+       apply elem_of_list_fmap in H0 as ((?&?)&?&?).
+       apply elem_of_list_lookup_1 in H1 as (?&?).
+       apply prefixes_from_ith_length in H1. simpl in H1.
+       rewrite /locale_of in EQ, H0.
+       rewrite length_app /= in H1. lia. }
+
+     iDestruct "IH" as (Ts) "(%DOM & WPS & CLOS)".
+     iExists (if decide (locale_of t e ∈ τs) then <[ locale_of t e := (e, Φ) ]> Ts else Ts).
+     iSplitR.
+     { iPureIntro. destruct decide.
+       - rewrite dom_insert_L. rewrite DOM.
+         rewrite union_comm_L. rewrite difference_union_L. set_solver.
+       - set_solver. }
+     destruct decide.
+     - iSplitL "WP WPS".
+       + rewrite big_sepM_insert.
+         2: { apply not_elem_of_dom. set_solver. }
+         iFrame. iSplitR.
+         { iPureIntro.
+           pose proof (from_locale_from_locale_of t [] efs e).
+           by rewrite app_nil_l app_nil_r in H0. }
+         iApply (big_sepM_impl with "[$]").
+         iModIntro. iIntros (k (e', Φ')) "%KTH".
+         simpl. rewrite decide_False; [set_solver| ].
+         intros <-. apply mk_is_Some, elem_of_dom in KTH. set_solver.
+       + iIntros "CLOS'".
+         rewrite big_sepM_insert.
+         2: { apply not_elem_of_dom. set_solver. }
+         iDestruct "CLOS'" as "((%EQ & WP2) & WPS2)".
+         rewrite wptp_from_gen_cons. iFrame.
+         iApply "CLOS". simpl.
+         iApply (big_sepM_impl with "[$]").
+         iModIntro. iIntros (k (e', Φ')) "%KTH".
+         rewrite decide_False; [set_solver| ].
+         intros <-. apply mk_is_Some, elem_of_dom in KTH. set_solver.
+     - iSplitL "WPS".
+       + simpl.
+         iApply (big_sepM_impl with "[$]").
+         iModIntro. iIntros (k (e', Φ')) "%KTH".
+         simpl. rewrite decide_False; [set_solver| ].
+         intros <-. apply mk_is_Some, elem_of_dom in KTH. set_solver.
+       + iIntros "CLOS'".
+         rewrite wptp_from_gen_cons. iSplitL "WP".
+         { iApply ("UPD" with "[] [$]").
+           iPureIntro. split; [| done].
+           rewrite locales_of_list_from_locales. simpl. set_solver. }
+         iApply "CLOS". simpl.
+         iApply (big_sepM_impl with "[$]").
+         iModIntro. iIntros (k (e', Φ')) "%KTH".
+         rewrite decide_False; [set_solver| ].
+         intros <-. apply mk_is_Some, elem_of_dom in KTH. set_solver.
+  Qed.
+
+
+Definition wptp_gen {Σ} W t Φs := (@wptp_from_gen Σ W [] t Φs).
